Switch to separation logic
Some core infrastructure (no cancel automation, and not all theorems are
immediately useful), as well as some examples in the form of separation
logic specs for TD.Read.

src/Disk.v
@@ -1,5 +1,6 @@
 Require Import Bytes.
 Require Export SepLogic.Mem.
+Require Import SepLogic.Pred.
 
 Definition addr := nat.
 
@@ -13,8 +14,10 @@ Opaque block.
 
 Record disk :=
   mkDisk { size: nat;
-           diskMem : mem addr block;
+           diskMem :> mem addr block;
            diskMem_domain: sized_domain diskMem size; }.
+
+Definition dpred := pred addr block.
 
 (* this coercion allows disks to be directly accessed with a function
 application: [d a] will implicitly call [disk_get d a] due to the coercion,
