src/SepLogic/Pred.v
@@ -1,0 +1,3 @@
+Require Export
+        SepLogic.Pred.Def
+        SepLogic.Pred.Ptsto.
