src/SepLogic/Pred/Def.v
@@ -1,0 +1,134 @@
+Require Import Automation.
+Require Import Setoid Classes.Morphisms.
+Require Import SepLogic.Mem.Def.
+
+Record pred A V :=
+  mkPred { pred_prop :> mem A V -> Prop }.
+
+Section Predicates.
+
+  Context {A V:Type}.
+  Implicit Types p q:pred A V.
+
+  Definition lift (P:Prop) : pred A V :=
+    mkPred (fun m => P /\ m = empty_mem).
+  Definition emp := lift True.
+  Definition exis X (P: X -> pred A V) :=
+    mkPred (fun m => exists x, P x m).
+
+  Definition ptsto (a:A) (v:V) : pred A V :=
+    mkPred (fun m => m a = Some v /\
+                  forall a', a <> a' -> m a' = None).
+
+  Definition star p q : pred A V :=
+    mkPred (fun m => exists m1 m2, p m1 /\
+                           q m2 /\
+                           mem_disjoint m1 m2 /\
+                           m = mem_union m1 m2).
+
+  Definition pimpl p q :=
+    forall m, p m -> q m.
+
+  Definition peq p q :=
+    pimpl p q /\ pimpl q p.
+
+  Notation "[| P |]" := (lift P) (at level 0).
+  Infix "*" := star.
+
+  Infix "===" := peq (no associativity, at level 70).
+  Infix "===>" := pimpl (no associativity, at level 70).
+
+  Lemma pimpl_refl : forall p, p ===> p.
+  Proof.
+    firstorder.
+  Qed.
+
+  Lemma pimpl_trans : forall p q r, p ===> q -> q ===> r -> p ===> r.
+  Proof.
+    firstorder.
+  Qed.
+
+  Add Parametric Relation :
+    (pred A V) pimpl
+      reflexivity proved by pimpl_refl
+      transitivity proved by pimpl_trans
+        as pimpl_rel.
+
+  Hint Resolve mem_disjoint_comm.
+  Hint Resolve mem_union_comm.
+
+  Hint Resolve mem_disjoint_from_union_1.
+  Hint Resolve mem_disjoint_from_union_2.
+  Hint Resolve mem_disjoint_both_to_union.
+  Hint Resolve mem_union_assoc.
+
+  Theorem star_comm : forall p q,
+      p * q === q * p.
+  Proof.
+    assert (forall p q, p * q ===> q * p).
+    unfold star, pimpl; simpl; intuition.
+    repeat deex.
+    descend; intuition eauto.
+
+    unfold peq; intuition.
+  Qed.
+
+  Theorem star_cancel : forall p1 p2 q1 q2,
+      p1 ===> p2 ->
+      q1 ===> q2 ->
+      p1 * q1 ===> p2 * q2.
+  Proof.
+    unfold star, pimpl; simpl; intros.
+    repeat deex.
+    descend; intuition eauto.
+  Qed.
+
+  Add Parametric Morphism : star
+      with signature peq ==> peq ==> peq
+        as star_mor.
+  Proof.
+    unfold peq; intuition auto using star_cancel.
+  Qed.
+
+  Add Parametric Morphism : star
+      with signature pimpl ==> pimpl ==> pimpl
+        as star_mor'.
+  Proof.
+    auto using star_cancel.
+  Qed.
+
+  Theorem star_assoc : forall p q r,
+      p * (q * r) === (p * q) * r.
+  Proof.
+    unfold star, peq, pimpl; simpl; intuition.
+    - repeat deex.
+      exists (mem_union m1 m0), m3; intuition eauto.
+      descend; intuition eauto.
+      eapply mem_disjoint_comm; eauto.
+      rewrite mem_union_assoc; eauto.
+    - repeat deex.
+      exists m0, (mem_union m3 m2); intuition eauto.
+      descend; intuition eauto.
+  Qed.
+
+  Theorem lift_extract : forall m P,
+      pred_prop [|P|] m -> P.
+  Proof.
+    unfold lift; simpl in *; intuition.
+  Qed.
+
+End Predicates.
+
+Notation "[| P |]" := (lift P) (at level 0) : pred_scope.
+Infix "*" := star : pred_scope.
+
+Infix "===" := peq (no associativity, at level 70) : pred_scope.
+Infix "===>" := pimpl (no associativity, at level 70) : pred_scope.
+
+Notation "'exists' x .. y , p" := (exis (fun x => .. (exis (fun y => p)) ..)) : pred_scope.
+
+Infix "|->" := ptsto (no associativity, at level 30) : pred_scope.
+
+Add Printing Coercion pred_prop.
+Delimit Scope pred_scope with pred.
+Notation "m |= F" := (pred_prop F%pred m) (at level 20, F at level 50).
