src/SepLogic/Pred/Ptsto.v
@@ -1,0 +1,14 @@
+Require Import Automation.
+
+Require Import SepLogic.Mem.Def.
+Require Import SepLogic.Pred.Def.
+
+Theorem ptsto_valid : forall `(m: mem A V) F a v,
+    m |= F * a |-> v ->
+    m a = Some v.
+Proof.
+  intros.
+  apply star_comm in H.
+  simpl in *; repeat deex.
+  unfold mem_union; simpl_match; auto.
+Qed.
