src/Shallow/TwoDiskProgTheorems.v
@@ -1,0 +1,123 @@
+Require Import SepLogic.
+Require Import Automation.
+Require Import Disk.
+
+Require Import Shallow.ProgLang.Hoare.
+Require Import Shallow.ProgLang.Prog.
+Require Import TwoDiskProg.
+
+Opaque pred_prop.
+
+Definition md_pred (md: option disk) (F: dpred) (P: Prop) :=
+  match md with
+  | Some d => d |= F
+  | None => P
+  end.
+
+Theorem md_pred_weaken : forall md F (P P':Prop),
+    md_pred md F P ->
+    (P -> P') ->
+    md_pred md F P'.
+Proof.
+  destruct md; intuition.
+Qed.
+
+Hint Resolve md_pred_weaken.
+
+Theorem Read0_ok : forall a,
+    prog_spec
+      (fun '(F0, F1, v0) state =>
+         {|
+           pre := md_pred (TD.disk0 state) (F0 * a |-> v0)%pred True /\
+                  md_pred (TD.disk1 state) F1 True;
+           post :=
+             fun r state' =>
+               match r with
+               | Working v => v = v0 /\
+                             md_pred (TD.disk0 state') (F0 * a |-> v0)%pred False /\
+                             md_pred (TD.disk1 state') F1 True
+               | Failed => md_pred (TD.disk0 state') (lift False) True /\
+                          md_pred (TD.disk1 state') F1 False
+               end;
+           crash :=
+             fun state' =>
+               md_pred (TD.disk0 state') (F0 * a |-> v0)%pred True /\
+               md_pred (TD.disk1 state') F1 True;
+         |})
+      (Prim (TD.Read d0 a))
+      TD.step.
+Proof.
+  unfold prog_spec; intros;
+    repeat match goal with
+           | [ H: context[let '(a, b) := ?p in _] |- _ ] =>
+             let a := fresh a in
+             let b := fresh b in
+             destruct p as [a b]
+           end;
+    simpl in *;
+    safe_intuition.
+  eapply (inversion_prim_exec H0); intros; eauto.
+  TD.inv_step.
+  inversion H2; subst; clear H2; simpl in *; repeat simpl_match; eauto.
+  destruct (TD.disk0 state') eqn:?; simpl in *; subst.
+  pose proof (ptsto_valid H).
+  unfold disk_get in *.
+  simpl_match; subst; intuition eauto.
+  destruct state'; simpl in *; subst; intuition eauto.
+  destruct disk1; simpl; intuition eauto.
+  pose proof (ptsto_valid H).
+  unfold disk_get in *.
+  simpl_match; subst; intuition eauto.
+  destruct v; subst; intuition eauto.
+  destruct (TD.disk0 state'); simpl in *; eauto.
+  apply lift_extract in H4; contradiction.
+Qed.
+
+Theorem Read1_ok : forall a,
+    prog_spec
+      (fun '(F0, F1, v0) state =>
+         {|
+           pre := md_pred (TD.disk0 state) F0 True /\
+                  md_pred (TD.disk1 state) (F1 * a |-> v0)%pred True;
+           post :=
+             fun r state' =>
+               match r with
+               | Working v => v = v0 /\
+                             md_pred (TD.disk0 state') F0 True /\
+                             md_pred (TD.disk1 state') (F1 * a |-> v0)%pred False
+               | Failed => md_pred (TD.disk0 state') F0 False /\
+                          md_pred (TD.disk1 state') (lift False) True
+               end;
+           crash :=
+             fun state' =>
+               md_pred (TD.disk0 state') F0 True /\
+               md_pred (TD.disk1 state') (F1 * a |-> v0)%pred True;
+         |})
+      (Prim (TD.Read d1 a))
+      TD.step.
+Proof.
+  unfold prog_spec; intros;
+    repeat match goal with
+           | [ H: context[let '(a, b) := ?p in _] |- _ ] =>
+             let a := fresh a in
+             let b := fresh b in
+             destruct p as [a b]
+           end;
+    simpl in *;
+    safe_intuition.
+  eapply (inversion_prim_exec H0); intros; eauto.
+  TD.inv_step.
+  inversion H2; subst; clear H2; simpl in *; repeat simpl_match; eauto.
+  destruct (TD.disk1 state') eqn:?; simpl in *; subst.
+  pose proof (ptsto_valid H1).
+  unfold disk_get in *.
+  simpl_match; subst; intuition eauto.
+  destruct state'; simpl in *; subst; intuition eauto.
+  destruct disk0; simpl; intuition eauto.
+  pose proof (ptsto_valid H1).
+  unfold disk_get in *.
+  simpl_match; subst; intuition eauto.
+  destruct v; subst; intuition eauto.
+  destruct (TD.disk1 state'); simpl in *; eauto.
+  apply lift_extract in H5; contradiction.
+Qed.
